policies/Compartments.v
@@ -1,0 +1,168 @@
+Require Import Coqlib.
+Require Import AST.
+Require Import Integers.
+Require Import Floats.
+Require Import Values.
+Require Import Ctypes.
+Require Import Cabs.
+Require Import String.
+Require Import Tags.
+Require Import Show.
+Require Import ExtLib.Structures.Monads. Import MonadNotation.
+
+Module Compartments <: Policy.
+  Import Passthrough.
+
+  Definition Comp : Type := ident.
+
+  Definition show_comp (C: Comp) : string :=
+    show (Zpos C).
+
+  Global Instance Show_comp : Show Comp :=
+  {| show := show_comp |}.
+
+
+  Variable init_comp : Comp.
+  
+  Inductive myVT :=
+  | LPtr (id:ident)
+  | SPtr (c:nat)
+  | N
+  .
+
+  Inductive myLT :=
+  | LMem (id:ident)
+  | SMem (c:nat)
+  | Free
+  .
+  
+  Definition val_tag := myVT.
+  Definition control_tag : Type := (Comp*nat).
+  Definition loc_tag := myLT.
+
+  Theorem vt_eq_dec : forall (t1 t2:val_tag), {t1 = t2} + {t1 <> t2}.
+  Proof. repeat decide equality. Qed.
+  Theorem ct_eq_dec : forall (t1 t2:control_tag), {t1 = t2} + {t1 <> t2}.
+  Proof. repeat decide equality. Qed.
+  Theorem lt_eq_dec : forall (t1 t2:loc_tag), {t1 = t2} + {t1 <> t2}.
+  Proof. repeat decide equality. Qed.
+
+  Definition def_tag : val_tag := N.
+  Definition InitPCT : control_tag := (init_comp, O).
+  Definition DefLT   : loc_tag := Free.
+  Definition DefHT   : loc_tag := Free.
+  Definition InitT   : val_tag := N.
+
+  Definition print_vt (t : val_tag) : string :=
+    match t with
+    | LPtr C => "Local " ++ show C
+    | SPtr c => "Shared " ++ show c
+    | N => "N"
+    end.
+
+  Definition print_ct (t : control_tag) : string :=
+    "Curr: " ++ show (fst t).
+  
+  Definition print_lt (t : loc_tag) : string :=
+    match t with
+    | LMem C => "Local " ++ show C
+    | SMem c => "Shared " ++ show c
+    | Free => "Free"
+    end.
+
+  Definition policy_state := unit.
+  Definition init_state : policy_state := tt.
+
+  Definition PolicyResult := PolicyResult policy_state.
+  Definition ltop := ltop lt_eq_dec policy_state.
+
+  Definition log := log policy_state.
+  
+  Definition color_eq (pt: val_tag) (lt: loc_tag) : bool :=
+    match pt, lt with
+    | Glob id1, Glob id2 => (id1 =? id2)%positive
+    | Dyn c1, Dyn c2 => (c1 =? c2)%nat
+    | _, _ => false
+    end.
+    
+  Definition inj_loc (s:string) (l:loc) : string :=
+    s ++ " at " ++ (print_loc l).
+
+  Local Open Scope monad_scope.
+  
+  Definition CallT (l:loc) (pct: control_tag) (fpt: val_tag) : PolicyResult control_tag :=
+
+
+  Definition LoadT (l:loc) (pct: control_tag) (pt vt: val_tag) (lts : list loc_tag) : PolicyResult val_tag :=
+    match pt with
+    | N => raise (PolicyFailure (inj_loc "PVI || LoadT X Failure" l))
+    | _ => if ltop.(forallb) (color_eq pt) lts then ret vt 
+           else raise (PolicyFailure (inj_loc "PVI || LoadT tag_eq_dec Failure" l))
+    end.
+
+  Definition StoreT (l:loc) (pct: control_tag) (pt vt: val_tag)
+    (lts : list loc_tag) : PolicyResult (control_tag * val_tag * list loc_tag) :=
+    match pt with
+    | N => raise (PolicyFailure (inj_loc "PVI || StoreT X Failure" l))
+    | _ => if ltop.(forallb) (color_eq pt) lts then ret (pct,vt,lts) 
+           else raise (PolicyFailure (inj_loc "PVI || StoreT tag_eq_dec Failure" l))
+    end.
+  
+  Definition BinopT (l:loc) (op : binary_operation) (pct: control_tag) (vt1 vt2 : val_tag) :
+    PolicyResult (control_tag * val_tag) :=
+    match vt1, vt2 with
+    | Dyn n, X =>  ret (pct, vt1)
+    | Glob id, X => ret (pct, vt1)
+    | _, _ => ret (pct, vt2)
+    end.
+
+  Definition ConstT (l:loc) (pct : control_tag) : PolicyResult val_tag := ret N.
+
+  Definition GlobalT (ce : composite_env) (id : ident) (ty : type) : val_tag * val_tag * loc_tag :=
+    (Glob id, N, Glob id).
+
+  Definition FunT (ce: composite_env) (id : ident) (ty : type) : val_tag := N.
+  
+  Definition LocalT (ce: composite_env) (l:loc) (pct : control_tag) (ty : type) :
+    PolicyResult (control_tag * val_tag * list loc_tag)%type :=
+    let c := pct in
+    ret (S c, Dyn c, ltop.(const) (Z.to_nat (sizeof ce ty)) (Dyn c)).
+  
+  Definition DeallocT (l:loc) (ce : composite_env) (pct : control_tag) (ty : type) :
+    PolicyResult (control_tag * val_tag * loc_tag) :=
+    ret (pct, N, N).
+
+  Definition MallocT (l:loc) (pct: control_tag) (fpt: val_tag) :
+    PolicyResult (control_tag * val_tag * val_tag * loc_tag * loc_tag) :=
+    log ("Malloc call at " ++ print_loc l ++ " associated with color " ++ print_ct pct);;
+    let c := pct in
+    ret (S c, Dyn c, N, Dyn c, Dyn c).
+
+  Definition FreeT (l:loc) (pct: control_tag) (pt: val_tag) (lts: list loc_tag) :
+    PolicyResult (control_tag * loc_tag) :=
+    ret (pct, N).
+
+  Definition ClearT (l:loc) (pct: control_tag) (pt: val_tag) (lt: loc_tag) :
+    PolicyResult loc_tag :=
+    ret N.
+  
+  (* Passthrough rules *)  
+  Definition CallT      := Passthrough.CallT policy_state val_tag control_tag.  
+  Definition ArgT       := Passthrough.ArgT policy_state val_tag control_tag.
+  Definition RetT       := Passthrough.RetT policy_state val_tag control_tag.
+  Definition AccessT    := Passthrough.AccessT policy_state val_tag control_tag.
+  Definition AssignT    := Passthrough.AssignT policy_state val_tag control_tag.
+  Definition CoalesceT  := Passthrough.CoalesceT policy_state val_tag vt_eq_dec.
+  Definition EffectiveT := Passthrough.EffectiveT val_tag def_tag. 
+  Definition UnopT      := Passthrough.UnopT policy_state val_tag control_tag.
+  Definition SplitT     := Passthrough.SplitT policy_state val_tag control_tag.
+  Definition LabelT     := Passthrough.LabelT policy_state control_tag.
+  Definition ExprSplitT := Passthrough.ExprSplitT policy_state val_tag control_tag.
+  Definition ExprJoinT  := Passthrough.ExprJoinT policy_state val_tag control_tag.
+  Definition FieldT     := Passthrough.FieldT policy_state val_tag control_tag.
+  Definition ExtCallT   := Passthrough.ExtCallT policy_state val_tag control_tag.
+  Definition PICastT    := Passthrough.PICastT policy_state val_tag control_tag loc_tag.
+  Definition IPCastT    := Passthrough.IPCastT policy_state val_tag control_tag loc_tag.
+  Definition PPCastT    := Passthrough.PPCastT policy_state val_tag control_tag loc_tag.
+  Definition IICastT    := Passthrough.IICastT policy_state val_tag control_tag.
+End PVI.
